scheduler/example/SCHMainA.v
@@ -1,0 +1,46 @@
+Require Import CRIS.
+Require Import CallFilter.
+Require Import SchHeader SchA.
+Require Import RRSHeader RRSA.
+Require Import NDSHeader NDSA.
+Require Import RRSNodeHeader RRSNodeA.
+Require Import NDSNodeHeader NDSNodeA.
+Require Import MemHeader MemA.
+Require Import SCHMainI.
+Set Implicit Arguments.
+
+Module SCHMainA. Section SCHMainA.
+  Context `{_crisG: !crisG Γ Σ α β τ _S _I, _concG: !concG}.
+  Context `{_schG: !SchA.newschG}.
+  Context `{_rrsG: !RRSA.rrsG}.
+  Context `{_ndsG: !NDSA.ndsG}.
+  Context `{_memG: !MemA.memG}.
+  Context `{_nodeG: !RRSNodeA.nodeG}.
+  Import SCHMainI.
+
+  Definition main_spec E : fspec :=
+    fspec_winv E
+      (fspec_simple (λ (_: unit),
+           ((λ arg, RRSAS.InitRRS ∗ RRSNodeAS.full_val (Vint 0) ∗ NDSA.InitNDS ∗ SchA.Tid 0 0)%I,
+            (λ ret, True)%I))).
+
+  Definition sp E : specmap :=
+    {[speckey_entry := fspec_to_rel (main_spec E)]}.
+
+  Definition fnsems (E : coPset) : fnsemmap :=
+    {[None := Some (msk_scp ∅ msk_true, (fsp_some (main_spec E), main))]}.
+
+  Program Definition smod E: SMod.t :=
+    {|
+      SMod.scopes := ∅;
+      SMod.fnsems := fnsems E;
+      SMod.initial_st := ∅;
+    |}.
+  Solve All Obligations with mod_tac.
+
+  Definition init_cond : iProp Σ :=
+    RRSAS.InitRRS ∗ RRSNodeAS.full_val (Vint 0) ∗ NDSA.InitNDS
+    ∗ own base_γ (gmap_view_frag 0 (DfracOwn 1) (to_agree 0)).
+
+  Definition t sp := SMod.to_mod sp (smod ⊤).
+End SCHMainA. End SCHMainA.
